update definitions and finish proofs

proof/definition_analysis/PRHL_Defs.ec
@@ -1,36 +1,989 @@
-require import AllCore Distr.
+require import AllCore Distr StdRing Real.
+
+import RField.
+
 
 (** pRHL characterisation  of leakage-freeness.
 
  Here we seek a characterisation of the leakage-free
  property in a pure probabilist Relational Hoare Logic
  formulation. The goal is to avoid handling explicitly
- the leakage, resorting instead to the EC's [sim]
- tactic.                                            *)
+ the leakage, resorting instead to the EC's pRHL
+ reasoning.                                      *)
 
 
 (** The setting:
 
- we consider a collection of Jasmin procedures that are
+ We consider a collection of Jasmin procedures that are
  extracted into EC in two modes ([XtrI] and [XtrR]).
  Each one of these is a module that includes the
- EC's model Jasmin-implemented functions:
+ EC's model of Jasmin-implemented functions:
 
-  - XtrI.f - an EC proc. that models the input/output
-      behaviour of Jasmin function [f] (hence, an
-      abstract or Ideal setting).
-  - XtrR.f - an EC proc.  that, in addition to the
+  - XtrI.f - an EC procedure modeling the input/output
+      behaviour of Jasmin function [f] (hence, calling
+      it an abstract or "Ideal" setting). This is
+      a stateless module (Jasmin do not allow global
+      variables).
+  - XtrR.f - an EC procedure that, in addition to the
       input/output behaviour, models also what is leaked
       during execution (accumulated in variable
       [XtrR.leakages]). This is what we call the
-      concrete or Real setting.
+      concrete or "Real" setting.
 
  As a meta-property of the extraction mechanism, we
  have that the behaviour of [XtrI.f] is indeed given
  by the marginal probability of [XtrR.f] (when the
  leakage is ignored). In any case, this fact is
- typically provable automatically with the [sim]
- tactic.                                           *)
+ typically proved automatically with the [sim]
+ tactic.
+
+ In what follows, we define an abstract theory [CT_Meta]
+ with wrappers that abstracts the Jasmin function under
+ consideration -- in there, [JI] and [JR] are
+ respectivelly wrappers of the abstract (ideal)
+ and concrete (real) extractions of the Jasmin
+ function.                                        *)
+
+
+(** This theory establishes the core definitions
+ and properties of the PRHL characterisation of
+ Leakage-freeness (what we call the CT-property,
+ as it extends the standard non-interference
+ based characterisation of the constant-time
+ property - here called ct-property).
+ In this theory, we focus on a single Jasmin
+ function [f]. Bellow, we shall establish
+ a compositionality result that ultimately justifies
+ this "local" focus.                           *)
+abstract theory CT_Meta.
+
+(** types for public and secret inputs, and output *)
+type pin_t, sin_t, out_t.
+
+(** This abstracts a single Jasmin function --
+ it will represent both the abstract (ideal) or
+ concrete (real) extracted variants.          *)
+module type JasminProcWrapper = {
+ proc main(pin: pin_t, sin: sin_t): out_t
+}.
+
+
+(** The CT-property can be understood as an
+ instance of the Real/Ideal paradigm. For a
+ given Jasmin function (abstracted by modules
+ [JI] and [JR], it establishes the equivalence
+ of the concrete (leaky) implementation with
+ abstract (pure) implementation combined with
+ simulated leakage. Both sides of the equivalence
+ are captured by the following modules [SimR]
+ and [RSim].                                *)
+ 
+
+
+(** [SimR] denotes the Simulated side of the
+ captured property (where leakage is simulated
+ resorting to the real implementation on
+ arbitrary secret inputs).                     *)
+module SimR(JI: JasminProcWrapper, JR: JasminProcWrapper) = {
+ proc main(pin: pin_t, sin sin': sin_t): out_t = {
+  var _r, r;
+  _r <@  JR.main(pin, sin');
+  r <@  JI.main(pin, sin);
+  return r;
+ }
+}.
+
+(** On the other side, the real (leaky)
+ implementation is conditioned by (a possibly
+ faulty) dummy simulator. This is a rather
+ artificial (technical) artifact to turn
+ the CT-property robust on possibly diverging
+ programs.                                     *)
+module RSim(JI: JasminProcWrapper)(JR: JasminProcWrapper) = {
+ proc main(pin: pin_t, sin: sin_t): out_t = {
+  var _r, r;
+  _r <@  JI.main(pin, sin); (* behaves as a dummy
+                             leakage simulator *)
+  r <@  JR.main(pin, sin);
+  return r;
+ }
+}.
+
+(** An apparently stronger variant of CT-property
+ is based on a more general variant [RSim]. As
+ we will see later, it turns out to be provably
+ equivalent to the former characterization.    *)
+module RSim'(JI: JasminProcWrapper)(JR: JasminProcWrapper) = {
+ proc main(pin: pin_t, sin sin': sin_t): out_t = {
+  var _r, r;
+  _r <@  JI.main(pin, sin');
+  r <@  JR.main(pin, sin);
+  return r;
+ }
+}.
+
+(** Another useful definition simplifies the
+ right-hand side (simulated) when it is known
+ that leakage does not depend on secret inputs
+ (standard non-interference). In that case,
+ running the simulator on arbitrary secret
+ inputs is indeed equivalent to run it with
+ the given secret inputs. We call this 
+ Coupled-Composition (CC). *)
+module CC(JI: JasminProcWrapper, JR: JasminProcWrapper) = {
+ proc main(pin: pin_t, sin: sin_t): out_t = {
+  var _r, r;
+  _r <@  JR.main(pin, sin);
+  r <@  JI.main(pin, sin);
+  return r;
+ }
+}.
+
+
+section.
+
+declare module JR <: JasminProcWrapper.
+declare module JI <: JasminProcWrapper {-JR}.
+
+declare axiom stateless_JI &m x: (glob JI){m} = x.
+
+declare axiom proj_JR_JI:
+ equiv [ JR.main ~ JI.main
+       : ={pin, sin} ==> ={res} ].
+
+
+lemma JI_JR_prE P &m _pin _sin:
+ Pr[ JI.main(_pin,_sin) @ &m : P res ]
+ = Pr[ JR.main(_pin,_sin) @ &m : P res ].
+proof. by rewrite eq_sym; byequiv proj_JR_JI. qed.
+
+(** STATELESS FACTS *)
+lemma JI_pr_m_m' P &m &m' _pin _sin:
+ Pr[ JI.main(_pin,_sin) @ &m : P res ]
+ = Pr[ JI.main(_pin,_sin) @ &m' : P res ].
+proof.
+byequiv (: _ ==> ={res}); simplify => //.
+by sim => /> *; apply stateless_JI.
+qed.
+
+lemma JR_pr_m_m' P &m &m' _pin _sin:
+ (glob JR){m} = (glob JR){m'} =>
+ Pr[ JR.main(_pin,_sin) @ &m : P (res,glob JR)]
+ = Pr[ JR.main(_pin,_sin) @ &m' : P (res,glob JR)].
+proof.
+move=> E_m_m'.
+byequiv (: ={pin,sin,glob JR} /\ pin{2}=_pin /\ sin{2}=_sin /\ (glob JR){1}=(glob JR){m} /\ (glob JR){2}=(glob JR){m'} ==> ={res, glob JR}); simplify => //.
+by sim => /> *.
+qed.
+
+lemma RSim_pr &m _pin _sin _rl:
+ Pr[RSim(JI,JR).main(_pin, _sin) @ &m : (res,glob JR)=_rl]
+ = Pr[JI.main(_pin, _sin) @ &m : true]
+   * Pr[JR.main(_pin, _sin) @ &m : (res,glob JR)=_rl].
+proof.
+byphoare (: pin=_pin /\ sin=_sin /\ (glob JR)=(glob JR){m} ==> (res,glob JR)=_rl) => //.
+proc; simplify.
+seq 1: (true)
+       Pr[JI.main(_pin, _sin) @ &m : true]
+       Pr[JR.main(_pin, _sin) @ &m : (res,glob JR)=_rl]
+       _ 0%r
+       (pin=_pin /\ sin=_sin /\ (glob JR) = (glob JR){m}) => //.
++ by call (:true) => //.
++ call (: pin = _pin /\ sin = _sin /\ (glob JR)=(glob JR){m} ==> true).
+   bypr; move=> /> &m' Hglob.
+   by apply (JI_pr_m_m' predT).
++ by auto.
++ call (: pin=_pin /\ sin=_sin /\ (glob JR)=(glob JR){m} ==> (res,glob JR)=_rl); last first.
+   by auto => /> /#.
+  bypr; move=> &m' [->] [->] Hglob.
+  byequiv => //.
+  proc* => //; simplify.
+  by call (:true); auto => /> * /#.
+qed.
+
+lemma RSim'_pr &m _pin _sin _sin' _rl:
+ Pr[RSim'(JI,JR).main(_pin, _sin, _sin') @ &m : (res,glob JR)=_rl]
+ = Pr[JI.main(_pin, _sin') @ &m : true]
+   * Pr[JR.main(_pin, _sin) @ &m : (res,glob JR)=_rl].
+proof.
+byphoare (: pin=_pin /\ sin=_sin /\ sin'=_sin' /\ (glob JR)=(glob JR){m} ==> (res,glob JR)=_rl) => //.
+proc; simplify.
+seq 1: (true)
+       Pr[JI.main(_pin, _sin') @ &m : true]
+       Pr[JR.main(_pin, _sin) @ &m : (res,glob JR)=_rl]
+       _ 0%r
+       (pin=_pin /\ sin=_sin /\ (glob JR) = (glob JR){m}) => //.
++ by call (:true) => //.
++ call (: pin = _pin /\ sin = _sin' /\ (glob JR)=(glob JR){m} ==> true).
+   bypr; move=> /> &m' Hglob.
+   by apply (JI_pr_m_m' predT).
++ by auto.
++ call (: pin=_pin /\ sin=_sin /\ (glob JR)=(glob JR){m} ==> (res,glob JR)=_rl); last first.
+   by auto => /> /#.
+  bypr; move=> &m' [->] [->] Hglob.
+  byequiv => //.
+  proc* => //; simplify.
+  by call (:true); auto => /> * /#.
+qed.
+
+lemma SimR_pr _pin _sin _sin' &m _rl:
+ Pr[SimR(JI, JR).main(_pin, _sin, _sin') @ &m : (res,glob JR)=_rl]
+ = Pr[JR.main(_pin, _sin') @ &m : (glob JR)=_rl.`2]
+   * Pr[JI.main(_pin, _sin) @ &m : res = _rl.`1].
+proof.
+byphoare (: pin=_pin /\ sin=_sin /\ sin'=_sin' /\ (glob JR)=(glob JR){m} ==> (res,glob JR)=_rl) => //.
+proc; simplify.
+seq 1: ((glob JR)=_rl.`2)
+       Pr[JR.main(_pin, _sin') @ &m : (glob JR)=_rl.`2]
+       Pr[JI.main(_pin, _sin) @ &m : res=_rl.`1]
+       _ 0%r
+       (pin=_pin /\ sin=_sin /\ sin'=_sin') => //.
++ by call (:true) => //.
++ call (: pin = _pin /\ sin = _sin' /\ (glob JR) = (glob JR){m} ==> (glob JR)=_rl.`2).
+   bypr; move=> &m' [->] [->] Hglob.
+   byequiv => //.
+   proc* => //.
+   by call (:true); auto => />.
++ by auto.
++ call (: pin=_pin /\ sin=_sin ==> res=_rl.`1); last by auto => /> /#.
+  bypr; move=> &m' [->] ->.
+  by apply (JI_pr_m_m' (pred1 _rl.`1)).
+hoare.
+by call (:true); auto => /#.
+qed.
+
+lemma CT_pr:
+ (* CT *)
+ equiv [ RSim(JI,JR).main ~ SimR(JI,JR).main
+       : ={pin, sin, glob JR} ==> ={res,glob JR} ]
+ <=>
+ (* CTpr *)
+ forall _pin _sin _sin' &m _rl,
+ Pr[ JI.main(_pin,_sin) @ &m : true ]
+ * Pr[ JR.main(_pin,_sin) @ &m : (res,glob JR)=_rl]
+ = Pr[ JI.main(_pin,_sin) @ &m : res=_rl.`1 ]
+   * Pr[ JR.main(_pin,_sin') @ &m : (glob JR)=_rl.`2 ].
+proof.
+split.
+ move => CT_J _pin _sin _sin' &m _rl.
+ by rewrite -RSim_pr mulrC -SimR_pr; byequiv CT_J => //=.
+move=> CTpr.
+bypr (res,glob JR){1} (res,glob JR){2} => //.
+move => &1 &2 _rl [->] [->] Eglob.
+rewrite /= RSim_pr SimR_pr (CTpr pin{2} sin{2} sin'{2} &1 _rl).
+rewrite (JI_pr_m_m' (pred1 _rl.`1) &1 &2) mulrC; congr => //.
+by rewrite (JR_pr_m_m' (fun x:_*_=>x.`2=_rl.`2) &1 &2).
+qed.
+
+lemma CT'_pr:
+ (* CT' *)
+ equiv [ RSim'(JI,JR).main ~ SimR(JI,JR).main
+       : ={pin, sin, glob JR} ==> ={res,glob JR} ]
+ <=>
+ (* CTpr *)
+ forall _pin _sin _sin1' _sin2' &m _rl,
+ Pr[ JI.main(_pin,_sin1') @ &m : true ]
+ * Pr[ JR.main(_pin,_sin) @ &m : (res,glob JR)=_rl]
+ = Pr[ JI.main(_pin,_sin) @ &m : res=_rl.`1 ]
+   * Pr[ JR.main(_pin,_sin2') @ &m : (glob JR)=_rl.`2 ].
+proof.
+split.
+ move => CT_J _pin _sin _sin1' _sin2' &m _rl.
+ by rewrite -RSim'_pr mulrC -SimR_pr; byequiv CT_J => //=.
+move=> CTpr.
+bypr (res,glob JR){1} (res,glob JR){2} => //.
+move => &1 &2 _rl [->] [->] Eglob.
+rewrite /= RSim'_pr SimR_pr (CTpr pin{2} sin{2} sin'{1} sin'{2} &1 _rl).
+rewrite (JI_pr_m_m' (pred1 _rl.`1) &1 &2) mulrC; congr => //.
+by rewrite (JR_pr_m_m' (fun x:_*_=>x.`2=_rl.`2) &1 &2).
+qed.
+
+
+(* Nice lemmas! but actually we do not rely on them...
+lemma JI_opsem1E &m:
+ exists d, forall _pin _sin &m' r,
+  Pr[JI.f(_pin, _sin) @ &m' : res=r]
+  = mu1 (d _pin _sin) r.
+proof.
+pose ff := fun (pin : pin_t) (sin : sin_t) (r : out_t)
+ => Pr[JI.f(pin, sin) @ &m : res = r].
+pose df := fun (pin : pin_t) (sin : sin_t) =>
+ mk (fun (x : out_t) => ff pin sin x).
+exists df => pin sin &m' r.
+rewrite -(JI_pr_m_m' (pred1 r) &m) /df muK /ff //=.
+apply Distr => /=; first smt(mu_bounded).
+move => l lU. 
+have ->: (StdBigop.Bigreal.BRA.big predT (fun (x : out_t) => Pr[JI.f(pin, sin) @ &m : res = x]) l)
+ = Pr[JI.f(pin, sin) @ &m : List.(\in) res l].
+ rewrite Pr [muE] (RealSeries.sumE_fin _ l) //=.
+  move=> x; apply contraR => Hx.
+  apply (eq_trans _ Pr[JI.f(pin, sin) @ &m : false]).
+   by rewrite Pr [mu_eq] /#. 
+  by rewrite Pr [mu_false].
+ apply StdBigop.Bigreal.BRA.eq_big_seq => x Hx /=.
+ by rewrite Pr [mu_eq] /#.
+smt(mu_bounded).
+qed.
+
+lemma JI_opsemE &m:
+ exists d, forall P _pin _sin &m',
+  Pr[JI.f(_pin, _sin) @ &m' : P res]
+  = mu (d _pin _sin) P.
+proof.
+have [dI EdI] := JI_opsem1E &m.
+exists dI => P pin sin &m'.
+rewrite Pr [muE] muE; apply RealSeries.eq_sum => x /=.
+case: (P x) => C.
+ by rewrite -(EdI _ _ &m') // Pr [mu_eq] /#.
+apply (eq_trans _ Pr[JI.f(pin, sin) @ &m' : false]).
+ by rewrite Pr [mu_eq] /#.
+by rewrite Pr [mu_false].
+qed.
+*)
+
+(** This is a workaroud for a current limitation of
+ EC's "rewrite Pr" mechanism. It can be
+ proved for concrete [JR] modules (see usage below). *)
+declare axiom prMuE P pin sin &m:
+ Pr[ JR.main(pin,sin) @ &m : P (res,glob JR)]
+ = RealSeries.sum (fun (x:_*_) => Pr [JR.main(pin,sin) @ &m : P (res,glob JR) /\ res=x.`1 /\ (glob JR)=x.`2]).
+
+lemma JR_opsem1E &m:
+ exists d, forall _pin _sin &m' (_rl:_*_),
+  (glob JR){m} = (glob JR){m'} =>
+  Pr[JR.main(_pin, _sin) @ &m' : (res,glob JR)=_rl]
+  = mu1 (d _pin _sin) _rl.
+proof.
+pose ff :=
+ fun pin sin (rl:_*_) => Pr[JR.main(pin, sin) @ &m : (res,glob JR)=rl].
+pose df := fun pin sin => mk (fun x => ff pin sin x).
+exists df => pin sin &m' rl Hmm'.
+rewrite (JR_pr_m_m' (pred1 rl) &m' &m) 1:/# /df muK /ff //=.
+apply Distr => /=; first smt(mu_bounded).
+move => xl xlU. 
+have ->: (StdBigop.Bigreal.BRA.big predT (fun x => Pr[JR.main(pin, sin) @ &m : (res,glob JR) = x]) xl)
+ = Pr[JR.main(pin, sin) @ &m : List.(\in) (res,glob JR) xl].
+ rewrite (prMuE (fun rl=>List.(\in) rl xl)%List _ _ &m).
+ rewrite (RealSeries.sumE_fin _ xl) //=.
+  move=> x; apply contraR => Hx.
+  apply (eq_trans _ Pr[JR.main(pin, sin) @ &m : false]).
+   by rewrite Pr [mu_eq] /#.
+  by rewrite Pr [mu_false].
+ apply StdBigop.Bigreal.BRA.eq_big_seq => x Hx /=.
+ by rewrite Pr [mu_eq] /#.
+smt(mu_bounded).
+qed.
+
+lemma JR_opsemE &m:
+ exists d, forall P _pin _sin &m',
+  (glob JR){m} = (glob JR){m'} =>
+  Pr[JR.main(_pin, _sin) @ &m' : P (res,glob JR)]
+  = mu (d _pin _sin) P.
+proof.
+have [dR EdR] := JR_opsem1E &m.
+exists dR => P pin sin &m' Hmm'.
+rewrite (prMuE P) muE.
+apply RealSeries.eq_sum => x /=.
+case: (P x) => C.
+ by rewrite -(EdR _ _ &m') // Pr [mu_eq] /#.
+apply (eq_trans _ Pr[JR.main(pin, sin) @ &m' : false]).
+ by rewrite Pr [mu_eq] /#.
+by rewrite Pr [mu_false].
+qed.
+
+lemma nosmt diverg_lemma pin sin &m:
+ (forall x, Pr[JR.main(pin, sin) @ &m : (res,glob JR)=x] = 0%r)
+ => Pr[JR.main(pin, sin) @ &m : true] = 0%r.
+proof.
+move=> eq0_pr; rewrite (prMuE predT) /predT /= RealSeries.sum0_eq //.
+by move=> x />; rewrite -(eq0_pr x) Pr [mu_eq] /#.
+qed.
+
+lemma CT_diverg:
+ (* CT *)
+ equiv [ RSim(JI,JR).main ~ SimR(JI,JR).main
+       : ={pin, sin, glob JR} ==> ={res, glob JR} ]
+ =>
+ (* divergence pattern cannot depend on secret inps *)
+ forall _pin _sin _sin' &m,
+ Pr[ JI.main(_pin,_sin) @ &m : true ] = 0%r
+ <=> Pr[ JI.main(_pin,_sin') @ &m : true ] = 0%r.
+proof.
+move => /CT_pr H _pin _sin _sin' &m.
+have HH: forall _pin _sin _sin' &m,
+   Pr[JI.main(_pin, _sin') @ &m : true] = 0%r
+   => Pr[JI.main(_pin, _sin) @ &m : true] = 0%r;
+last by smt().
+clear _pin _sin _sin' &m => _pin _sin _sin' &m.
+rewrite !(JI_JR_prE predT) /predT /= => Hsin'.
+have {H}H: forall _rl,
+ Pr[JR.main(_pin, _sin) @ &m : (res,glob JR) = _rl] = 0%r.
+ move=> _rl; move: (H _pin _sin _sin' &m _rl); move=> {H}.
+ have ->/=: Pr[JR.main(_pin, _sin') @ &m : (glob JR) = _rl.`2] = 0%r by smt(mu_sub mu_bounded).
+ rewrite (JI_JR_prE predT) /predT /=.
+ have: Pr[JR.main(_pin, _sin) @ &m : (res,glob JR) = _rl] <= Pr[JR.main(_pin, _sin) @ &m : true] by smt(mu_sub).
+ smt(mu_bounded).
+by rewrite (prMuE predT) RealSeries.sum0_eq //= /#.
+qed.
+
+lemma ct_pr:
+ (* ct *)
+ equiv [ JR.main ~ JR.main
+       : ={pin, glob JR} ==> ={glob JR} ]
+ <=>
+ (* ctpr *)
+ forall _pin _sin _sin' &m _l,
+  Pr[ JR.main(_pin,_sin) @ &m : (glob JR)=_l]
+  = Pr[ JR.main(_pin,_sin') @ &m : (glob JR)=_l ].
+proof.
+split.
+ move => ct_J _pin _sin _sin' &m _l.
+ by byequiv ct_J => // /#.
+move=> ctpr.
+bypr (glob JR){1} (glob JR){2} => //.
+move => &1 &2 _l [-> E].
+rewrite (JR_pr_m_m' (fun x:_*_=>x.`2=_l) &1 &2) //=.
+by apply ctpr.
+qed.
+
+(** CT implies the standard non-interference property
+  that ensures that secret inputs are not leaked *)
+lemma CT_ct:
+ (* CT *)
+ equiv [ RSim(JI,JR).main ~ SimR(JI,JR).main
+       : ={pin, sin, glob JR} ==> ={res, glob JR} ]
+ =>
+ (* ct *)
+ equiv [ JR.main ~ JR.main
+       : ={pin, glob JR} ==> ={glob JR} ].
+proof.
+rewrite CT_pr ct_pr => CT pin sin sin' &m _l.
+case: (exists x, 0%r < Pr[JI.main(pin, sin) @ &m : res = x]).
+ move => [r Hr].
+ have XX: forall _sin',
+   Pr[JR.main(pin, _sin') @ &m : (glob JR) = _l]
+   = Pr[JR.main(pin, sin) @ &m : (res,glob JR)=(r,_l)]
+     * Pr[JI.main(pin, sin) @ &m : true]
+     / Pr[JI.main(pin, sin) @ &m : res = r].
+  move => _sin'.
+  move: (CT pin sin _sin' &m (r,_l)) => E; field E; smt().
+ by rewrite (XX sin) (XX sin') /#.
+case: (exists x, 0%r < Pr[JI.main(pin, sin') @ &m : res = x]).
+ move => [r Hr].
+ have XX: forall _sin,
+   Pr[JR.main(pin, _sin) @ &m : (glob JR) = _l]
+   = Pr[JR.main(pin, sin') @ &m : (res,glob JR)=(r,_l)]
+     * Pr[JI.main(pin, sin') @ &m : true]
+     / Pr[JI.main(pin, sin') @ &m : res = r].
+  move => _sin.
+  move: (CT pin sin' _sin &m (r,_l)) => E; field E; smt().
+ by rewrite (XX sin'); rewrite (XX sin); smt().
+rewrite !negb_exists /= => T1 T2.
+have {T1}I1: forall a, Pr[JI.main(pin, sin') @ &m : res = a]=0%r.
+ by move=> a; move: (T1 a); smt(mu_bounded).
+have {T2}I2: forall a, Pr[JI.main(pin, sin) @ &m : res = a]=0%r.
+ by move=> a; move: (T2 a); smt(mu_bounded).
+have R1: Pr[JR.main(pin, sin') @ &m : true] = 0%r.
+ apply (diverg_lemma pin sin' &m); move => [r rl].
+ pose X:= Pr[JR.main(_,_) @ &m : (res,glob JR)=_].
+ have: X <= Pr[JR.main(pin, sin') @ &m : res=r] by smt(mu_sub).
+ rewrite -(JI_JR_prE (pred1 r)) /pred1 /X /= (I1 r); smt(mu_bounded).
+have R2: Pr[JR.main(pin, sin) @ &m : true] = 0%r.
+ apply (diverg_lemma pin sin &m); move => [r rl].
+ pose X:= Pr[JR.main(_,_) @ &m : (res,glob JR)=_].
+ have: X <= Pr[JR.main(pin, sin) @ &m : res=r] by smt(mu_sub).
+ rewrite -(JI_JR_prE (pred1 r)) /pred1 /X /= (I2 r); smt(mu_bounded).
+smt(mu_sub mu_bounded).
+qed.
+
+(* From the non-interference property, we strengthen
+ the previously established independence of divergence
+ from secret inputs. Indeed, the probability of
+ termination is also insensitive to secret inputs. *)
+lemma ct_pr_term:
+ (* ct *)
+ equiv [ JR.main ~ JR.main
+       : ={pin, glob JR} ==> ={glob JR} ]
+ =>
+ (* pr_term *)
+ forall _pin _sin _sin' &m,
+ Pr[ JI.main(_pin,_sin) @ &m : true]
+ = Pr[ JI.main(_pin,_sin') @ &m : true ].
+proof.
+move => /ct_pr Hct _pin _sin _sin' &m.
+have [dR HdR]:= JR_opsemE &m.
+rewrite !(JI_JR_prE predT) /predT /=.
+rewrite (HdR predT _ _ &m) //.
+rewrite (HdR predT _ _ &m) //.
+have: dsnd (dR _pin _sin) = dsnd (dR _pin _sin').
+ rewrite eq_distr => l.
+ rewrite !dmap1E /pred1 /(\o) /=.
+ rewrite -(HdR _ _ _ &m) // -(HdR _ _ _ &m) //=.
+ by apply Hct.
+smt(weight_dmap).
+qed.
+
+(* It allow us to recover (an essentially equivalent
+  formulation of the) original Leakage-Free definition *)
+lemma CT_LF &m':
+ (* CT *)
+ equiv [ RSim(JI,JR).main ~ SimR(JI,JR).main
+       : ={pin, sin, glob JR} ==> ={res, glob JR} ]
+ =>
+ (* LF *)
+ exists f,
+  forall pin sin &m rl,
+   (glob JR){m} = (glob JR){m'} =>
+   let v = Pr[ JR.main(pin,sin) @ &m : (res,glob JR)=rl ] in
+   let w = Pr[ JR.main(pin,sin) @ &m : res=rl.`1 ] in
+   0%r < w =>
+   v / w = f pin rl.`2.
+proof.
+move => CT.
+have /ct_pr_term E:= CT_ct CT.
+pose f := fun pin l =>
+           Pr[JR.main(pin,witness) @ &m' : (glob JR)=l]
+           / Pr[JI.main(pin,witness) @ &m' : true].
+exists f => pin sin &m [r l] Eg @/f /=.
+rewrite CT_pr in CT.
+have {CT}/=CT:= (CT pin sin witness &m (r,l)).
+rewrite -(JR_pr_m_m' (fun x:_*_=>x.`2=l) &m &m') //=.
+rewrite -(JI_pr_m_m' predT &m).
+rewrite -!(JI_JR_prE (pred1 r)) /pred1 /= => Hw.
+rewrite -(E pin sin witness); field CT;
+smt(mu_sub mu_bounded).
+qed.
+
+(** Moreover, we get an equivalence from CT to
+  a (apparently) more general definition CT' where
+  the "dummy call" on the left-hand side is
+  called with arbitrary secret inputs.       *)
+lemma CT_CT':
+ (* CT *)
+ equiv [ RSim(JI,JR).main ~ SimR(JI,JR).main
+       : ={pin, sin, glob JR} ==> ={res, glob JR} ]
+ <=>
+ (* CT' *)
+ equiv [ RSim'(JI,JR).main ~ SimR(JI,JR).main
+       : ={pin, sin, glob JR} ==> ={res, glob JR} ].
+proof.
+split.
+ move=> CT; have ct:= CT_ct CT.
+ move: CT; rewrite CT_pr CT'_pr.
+ move => CT pin sin sin1' sin2' &m rl.
+ rewrite (ct_pr_term ct _ _ sin).
+ by apply CT.
+rewrite CT_pr CT'_pr => CT' pin sin sin' &m rl.
+by apply CT'.
+qed.
+
+(** Of course, non-interference, which is often
+  trivial to establish, allows us to simplify CT
+  by factoring out the "independence on secret
+  inputs". *)
+lemma ct_CC_CT:
+ (* ct *)
+ equiv [ JR.main ~ JR.main
+       : ={pin, glob JR} ==> ={glob JR} ]
+ /\
+ (* CC *)
+ equiv [ RSim(JI,JR).main ~ CC(JI,JR).main
+       : ={pin, sin, glob JR}
+         ==> ={res, glob JR} ]
+ <=>
+ (* CT *)
+ equiv [ RSim(JI,JR).main ~ SimR(JI,JR).main
+       : ={pin, sin, glob JR}
+         ==> ={res, glob JR} ].
+proof.
+split.
+ (* ct /\ CC => CT *)
+ move => [ct_JR CC_J].
+ transitivity CC(JI,JR).main
+  ( ={pin, sin, glob JR} ==> ={res, glob JR} )
+  ( ={pin, sin, glob JR} ==> ={res, glob JR} ) => //.
+  move=> /> &1 &2 -> ->.
+  by exists (glob JR){2} (pin,sin){2} => /#.
+ proc.
+ call (:true).
+ call ct_JR.
+ by auto => /> &1 &2; apply stateless_JI.
+(* CT => ct /\ CC *)
+move=> CT_J; rewrite -andaE; split.
+ by apply CT_ct.
+(* CT /\ ct => CC *)
+move=> ct_J.
+transitivity SimR(JI,JR).main
+ (={pin, sin, glob JR} ==> ={res, glob JR})
+ (={pin, sin, glob JR} ==> ={res, glob JR}) => //.
+ by move => /> &1 &2 -> ->; exists (glob JR){2} (pin{2},sin{2},witness) => /#.
+proc.
+call (:true).
+call ct_J; auto => />.
+smt(stateless_JI).
+qed.
+
+
+(* DETERMINISTIC FUNCTIONALITIES
+
+  Moreover, if we exclude the non-determinism
+  from the functionalities, we recover back the
+  standard non-interference characterisation of
+  constant-time.
+
+  Notice that here we adopt a notion of determinism
+  which is fairly weak:
+    1) it does not entail termination (uses partiall HL triples)
+    2) it only concerns the functionality (is independent of the leakage)
+
+  This makes it easier to prove (e.g. by resorting to
+  established correctness lemmas), or to be handled
+  by some externally trusted annotation (e.g. established
+  by a simple type system -- notice that sources of
+  non-determinism in Jasmin are fairly restricted). Notice that the burden on statically check
+  non-determinism is much lower that full termination (safety) check.
+ *)
+lemma JI_det f _pin _sin:
+ (* det *)
+ hoare [ JI.main : pin=_pin /\ sin=_sin ==> res = f _pin _sin ]
+ =>
+ forall &m r,
+   Pr[JI.main(_pin, _sin) @ &m : res = r ]
+   = Pr[JI.main(_pin, _sin) @ &m : r = f _pin _sin ].
+proof.
+move => Hdet &m r.
+byequiv (: ={pin,sin} /\ pin{2}=_pin /\ sin{2}=_sin ==> _) => //.
+conseq (: ={pin, sin} ==> true)
+       (: pin=_pin /\ sin=_sin ==> res = f _pin _sin)
+       _ => //=.
+by sim; smt(stateless_JI).
+qed.
+
+lemma JR_det f _pin _sin:
+ (* det *)
+ hoare [ JI.main : pin=_pin /\ sin=_sin ==> res = f _pin _sin ]
+ =>
+ forall &m l,
+   Pr[JR.main(_pin, _sin) @ &m : (glob JR) = l]
+   = Pr[JR.main(_pin, _sin) @ &m : (res,glob JR) = (f _pin _sin, l) ].
+proof.
+move => Hdet &m rl.
+rewrite eq_sym.
+byequiv (: ={pin,sin,glob JR} /\ pin{2}=_pin /\ sin{2}=_sin ==> _) => //.
+conseq (: ={pin, sin, glob JR} ==> ={glob JR})
+       (: pin=_pin /\ sin=_sin  ==> res = f _pin _sin)
+       _ => //=.
+ by conseq proj_JR_JI Hdet => /> /#.
+by sim => /> *; apply stateless_J.
+qed.
+
+
+lemma ct_det_CT:
+ (* ct *)
+ equiv [ JR.main ~ JR.main
+       : ={pin, glob JR} ==> ={glob JR} ]
+ (* det *)
+ =>
+ (exists f, forall _pin _sin,
+   hoare [ JI.main : pin=_pin /\ sin=_sin ==> res = f _pin _sin ])
+ (* CT *)
+ => 
+ equiv [ RSim(JI,JR).main ~ SimR(JI,JR).main
+       : ={pin, sin, glob JR} ==> ={res, glob JR} ].
+proof.
+rewrite CT_pr ct_pr => ct_j [f Hf] pin sin sin' &m rl.
+move: (Hf pin sin) => {Hf} Hf.
+case: (rl.`1 = f pin sin) => E.
+ rewrite (JI_det _ _ _ Hf &m) E /=; congr.
+ by rewrite -(ct_j pin sin sin' &m) (JR_det _ _ _ Hf &m) -E /#.
+rewrite (JI_det _ _ _ Hf &m) E Pr [mu_false] /=.
+have ?: Pr[JR.main(pin, sin) @ &m : res = rl.`1] = 0%r.
+ rewrite -(JI_JR_prE (pred1 rl.`1) &m) /pred1 /= (JI_det _ _ _ Hf &m).
+ by rewrite E Pr [mu_false].
+have ->//: Pr[JR.main(pin, sin) @ &m : (res,glob JR)=rl] = 0%r.
+apply (eq_trans _ Pr[JR.main(pin, sin) @ &m : res = rl.`1 /\ (glob JR) = rl.`2]). 
+ smt(mu_sub).
+smt(mu_sub mu_bounded).
+qed.
+
+(** In most cases, the pattern of non-termination
+  is fully determined by public inputs. In that case,
+  we get a simpler (and much more intuitive) definition of CT.
+*)
+
+(* Assertin failed
+pred pinll = exists f_ll, forall _pin,
+ phoare [JI.f : pin=_pin ==> true ] = (b2r (f_ll _pin)).
+*)
+lemma pinll_pr:
+ (* pinll *)
+ (exists f_ll, forall _pin,
+  phoare [JI.main : pin=_pin ==> true ] = (b2r (f_ll _pin)))
+ <=>
+ exists (pin_ll: pin_t -> bool), forall pin sin &m, Pr[ JI.main(pin, sin) @ &m : true ] = (b2r (pin_ll pin)).
+proof.
+split; move=> [fpinll Hpinll]; exists fpinll.
+ by move => pin sin &m; byphoare (Hpinll pin). 
+move=> pin.
+by bypr => /#.
+qed.
+
+lemma pinll_RSim:
+ (* pinll *)
+ (exists f_ll, forall _pin,
+  phoare [JI.main : pin=_pin ==> true ] = (b2r (f_ll _pin)))
+ =>
+ equiv [ RSim(JI,JR).main ~ JR.main
+       : ={pin, sin, glob JR} ==> ={res, glob JR} ].
+proof.
+move => /pinll_pr [fll Hll].
+bypr (res,glob JR){1} (res,glob JR){2} => //.
+move => /> &1 &2 rl -> -> Eg.
+rewrite RSim_pr Hll.
+case: (fll pin{2}) => //= C.
+ by rewrite (JR_pr_m_m' (pred1 rl) &1 &2) //.
+move: (Hll pin{2} sin{2} &2); rewrite C b2r0.
+rewrite (JI_JR_prE predT).
+smt(mu_sub mu_bounded).
+qed.
+
+(* Combining previously established results we
+ get what is perhaps simpler path to establish
+ CT for non-deterministic programs (in most common
+ cases).
+
+   1 - establish termination;
+   2 - prove standard non-interference
+   3 - establish Coupled-Composition
+        ( r <@ fR  ~  _ <@ fR; r <@ fI )
+ *)
+lemma pinll_ct_CC_CT:
+ (* pinll *)
+ (exists f_ll, forall _pin,
+  phoare [JI.main : pin=_pin ==> true ] = (b2r (f_ll _pin)))
+ =>
+ (* ct *)
+ equiv [ JR.main ~ JR.main
+       : ={pin, glob JR} ==> ={glob JR} ]
+ /\
+ (* CC *)
+ equiv [ JR.main ~ CC(JI,JR).main
+       : ={pin, sin, glob JR}
+         ==> ={res, glob JR} ]
+ <=> 
+ (* CT *)
+ equiv [ RSim(JI,JR).main ~ SimR(JI,JR).main
+       : ={pin, sin, glob JR} ==> ={res, glob JR} ].
+proof.
+move => pinll; split.
+ move=> [ct CC].
+ rewrite -ct_CC_CT; split => //.
+ transitivity JR.main
+   (={pin, sin, glob JR} ==> ={res, glob JR})
+   (={pin, sin, glob JR} ==> ={res, glob JR}) => //.
+  by move => /> &1 &2 -> ->; exists (glob JR){2} (pin,sin){2} => /#.
+ by apply pinll_RSim.
+rewrite -ct_CC_CT; move => [ct SC]; split => //.
+transitivity RSim(JI, JR).main
+   (={pin, sin, glob JR} ==> ={res, glob JR})
+   (={pin, sin, glob JR} ==> ={res, glob JR}) => //.
+ by move => /> &1 &2 -> ->; exists (glob JR){2} (pin,sin){2} => /#.
+by symmetry; conseq (pinll_RSim pinll) => /#.
+qed.
+
+end section.
+
+end CT_Meta.
+
+(** We now address compositionality (the secret output
+ of one function is passed to the secret inputs of
+ some other function. For this, we critically rely
+ on the strong (equivalent) variant of CT (what we
+ have called CT').                                 *)
+theory CT_Comp.
+
+type pin1_t, pin2_t, sin1_t, sin2_t, out1_t, out2_t.
+
+clone CT_Meta as F1
+ with type pin_t <- pin1_t,
+      type sin_t <- sin1_t,
+      type out_t <- out1_t.
+
+clone CT_Meta as F2
+ with type pin_t <- pin2_t,
+      type sin_t <- out1_t * sin2_t,
+      type out_t <- out2_t.
+
+type pin_t = pin1_t * pin2_t.
+type sin_t = sin1_t * sin2_t.
+clone CT_Meta as F
+ with type pin_t <- pin_t,
+      type sin_t <- sin_t,
+      type out_t <- out2_t.
+
+(* we need to combine the two procs, otherwise,
+ we... *)
+module type Jasmin2ProcWrapper = {
+ proc f1(pin: pin1_t, sin: sin1_t): out1_t
+ proc f2(pin: pin2_t, sin: out1_t*sin2_t): out2_t
+}.
+
+module Proc1 (J: Jasmin2ProcWrapper): F1.JasminProcWrapper = {
+ proc main = J.f1
+}.
+
+module Proc2 (J: Jasmin2ProcWrapper): F2.JasminProcWrapper = {
+ proc main = J.f2
+}.
+
+module FComp (J1: F1.JasminProcWrapper)(J2: F2.JasminProcWrapper): F.JasminProcWrapper = {
+ proc main(pin: pin_t, sin: sin_t): out2_t = {
+  var pin1, pin2, sin1, sin2, r1, r2;
+  (pin1, pin2) <- pin;
+  (sin1, sin2) <- sin;
+  r1 <@ J1.main(pin1, sin1);
+  r2 <@ J2.main(pin2, (r1,sin2));
+  return r2;
+ }
+}.
+
+section.
+
+declare module JR <: Jasmin2ProcWrapper.
+module JR1 = Proc1(JR).
+module JR2 = Proc2(JR).
+(*
+declare module JR1 <: F1.JasminProcWrapper.
+declare module JR2 <: F2.JasminProcWrapper {-JR1}.
+(*obs: doesn't work!!!
+(* A note about (glob JR1) and (glob JR2): These modules
+ are expected to accumulate the leakage in a global variable.
+ Hence, they share the state. This justifies why we
+ shall only look only at (glob JR2), and add the
+ axiom [globJR_eq] establishing their equality. Again,
+ this axiom can be easily discharged during instantiation. *) 
+declare axiom globJR_eq &1 &2:
+ (glob JR1){1}=(glob JR1){2} <=> (glob JR2){1}=(glob JR2){2}.
+*)
+*)
+
+declare module JI1 <: F1.JasminProcWrapper {-JR}.
+declare module JI2 <: F2.JasminProcWrapper {-JI1, -JR}.
+
+declare axiom stateless_JI1 &m x: (glob JI1){m} = x.
+declare axiom stateless_JI2 &m x: (glob JI2){m} = x.
+declare axiom proj_JR_JI1:
+ equiv [ JR1.main ~ JI1.main
+       : ={pin, sin} ==> ={res} ].
+declare axiom proj_JR_JI2:
+ equiv [ JR2.main ~ JI2.main
+       : ={pin, sin} ==> ={res} ].
+declare axiom prMuE1 P pin sin &m:
+ Pr[ JR1.main(pin,sin) @ &m : P (res,glob JR1)]
+ = RealSeries.sum (fun (x:_*_) => Pr [JR1.main(pin,sin) @ &m : P (res,glob JR1) /\ res=x.`1 /\ (glob JR1)=x.`2]).
+declare axiom prMuE2 P pin sin &m:
+ Pr[ JR2.main(pin,sin) @ &m : P (res,glob JR2)]
+ = RealSeries.sum (fun (x:_*_) => Pr [JR2.main(pin,sin) @ &m : P (res,glob JR2) /\ res=x.`1 /\ (glob JR2)=x.`2]).
+
+lemma Compositionality:
+ (* CT *)
+ equiv [ F1.RSim(JI1,JR1).main ~ F1.SimR(JI1,JR1).main
+       : ={pin, sin, glob JR1} ==> ={res,glob JR1} ]
+ =>
+ (* CT *)
+ equiv [ F2.RSim(JI2,JR2).main ~ F2.SimR(JI2,JR2).main
+       : ={pin, sin, glob JR2} ==> ={res,glob JR2} ]
+ =>
+ (* CT *)
+ equiv [ F.RSim(FComp(JI1,JI2),FComp(JR1,JR2)).main ~ F.SimR(FComp(JI1,JI2),FComp(JR1,JR2)).main
+       : ={pin, sin, glob FComp(JR1,JR2)} ==> ={res,glob FComp(JR1,JR2)} ].
+proof.
+rewrite (F1.CT_CT' JR1 JI1 stateless_JI1 proj_JR_JI1 prMuE1) => CT1.
+rewrite (F2.CT_CT' JR2 JI2 stateless_JI2 proj_JR_JI2 prMuE2) => CT2.
+proc*; simplify.
+inline F.RSim(FComp(JI1, JI2), FComp(JR1, JR2)).main.
+inline FComp(JI1, JI2).main FComp(JR1, JR2).main.
+transitivity {1}
+ { pin10 <- pin.`1;
+   pin2 <- pin.`2;
+   sin10 <- sin.`1;
+   sin2 <- sin.`2;
+   r10 <@ JI1.main(pin10, sin10);
+   r1 <@ JR1.main(pin10, sin10);
+   r <@ F2.RSim'(JI2,JR2).main(pin2,(r1,sin2),(r10,sin2)); }
+ ( ={pin, sin, glob JR2, glob JR1} ==> ={r, glob JR2, glob JR1} )
+ ( ={pin, sin, glob JR2, glob JR1} ==> ={r, glob JR2, glob JR1} ) => //.
++ by move=> /> &2; exists (glob JR){2} pin{2} sin{2} => //.
++ inline F2.RSim'(JI2, JR2).main.
+  swap {2} 2 4.
+  swap {2} 3 4.
+  swap {2} 8 2.
+  swap {2} [5..9] -1.
+  swap {1} [10..13] -3.
+  wp; call (: true).
+  wp; call (: true).
+  wp; call (: true).
+  wp; call (: true).
+  auto => /> *.
+  smt(stateless_JI1 stateless_JI2).
+inline F.SimR(FComp(JI1, JI2), FComp(JR1, JR2)).main.
+inline FComp(JR1, JR2).main FComp(JI1, JI2).main.
+swap {1} 2 1.
+swap {1} [3..4] 2.
+swap {2} [9..10] 5.
+seq 4 13: (#pre /\ r1{1}=r10{2} /\ (pin2=pin.`2){2} /\ (pin20=pin.`2){2} /\ (sin2=sin'.`2){2} /\ (sin20=sin.`2){2}).
++ transitivity {1}
+   { r1 <@ F1.RSim'(JI1, JR1).main(pin.`1,sin.`1, sin.`1); }
+   ( ={pin, sin, glob JR2, glob JR1}
+     ==> ={pin, sin, glob JR2, glob JR1, r1} )
+   ( ={pin, sin, glob JR2, glob JR1}
+     ==> ={pin, sin, glob JR2, glob JR1} /\
+        r1{1} = r10{2} /\ pin2{2} = pin{2}.`2 /\ sin2{2} = sin'{2}.`2 /\
+        pin20{2} = pin{2}.`2 /\ sin20{2} = sin{2}.`2) => //.
+  - by move => /> &2; exists (glob JR){2} pin{2} sin{2}.
+  - by inline *; sim; auto => />; smt(stateless_JI1).
+  transitivity {2}
+   { r10 <@ F1.SimR(JI1,JR1).main(pin.`1,sin.`1,sin'.`1); }
+   ( ={pin, sin, glob JR2, glob JR1}
+     ==> ={pin, sin, glob JR2, glob JR1} /\ r1{1}=r10{2} )
+   ( ={pin, sin, sin', glob JR2, glob JR1}
+     ==> ={pin, sin, glob JR2, glob JR1, r10} /\
+        pin2{2} = pin{2}.`2 /\ sin2{2} = sin'{2}.`2 /\
+        pin20{2} = pin{2}.`2 /\ sin20{2} = sin{2}.`2)
+ => //.
+  - by move => /> &2; exists (glob JR){2} pin{2} sin{2} sin'{2}.
+  - move => />.
+  - by call CT1 => //.
+  inline*.
+  wp; call (: true).
+  wp; call (: true).
+  auto => /> *; smt(stateless_JI1).
+transitivity {2}
+ { r <@ F2.SimR(JI2,JR2).main(pin.`2,(r10,sin.`2), (r1,sin'.`2)); }
+ ( ={pin, sin, glob JR2, glob JR1} /\ r1{1}=r10{2}
+     ==> ={r, glob JR2, glob JR1} )
+ ( ={pin, sin, sin', glob JR2, glob JR1, r1, r10} /\
+   pin2{2} = pin{2}.`2 /\ sin2{2} = sin'{2}.`2 /\
+   pin20{2} = pin{2}.`2 /\ sin20{2} = sin{2}.`2
+   ==> ={glob JR2, glob JR1, r} ) => //.
+- by move => /> &2; exists (glob JR){2} pin{2} r1{2} r10{2} sin{2} sin'{2}.
+- by call CT2; auto => /> //.
+inline*.
+wp; call (: true).
+wp; call (: true).
+auto => /> *; smt(stateless_JI2).
+qed.
+
+end section.
+
+end CT_Comp.
+
+
+(*
+(* testing instantiation...
+
+  obs: this is for testing purposes only -- the actual
+ proofs shall appear in a separate file...         *)
 
 from Jasmin require import JModel.
 require W64_SchnorrExtract.
@@ -42,810 +995,202 @@ module XtrI = W64_SchnorrExtract.M(W64_SchnorrExtract.Syscall).
 require import Array256 Array32 WArray256.
 
 
-(** Leakage-freeness:
+theory Bn_rsample.
 
- The characterisation of leakage-freeness in the
- pRHL setting is roughly framed in the Simulation
- paradigm. Intuitively, we shall ask the Real-word
- [XtrR.f] to be simulated by the Ideal-word [XtrI.f]
- and a simulator that has only access to the public
- inputs of [f]. Moreover, we take the simulator to be
- constructed by running the "real" implementation
- itself with arbitrary secret inputs.
+clone import CT_Meta as Bn_rsample_CT
+ with type pin_t <- W64.t Array32.t,
+      type sin_t <- unit,
+      type out_t <- W64.t Array32.t.
 
- Consider the module:
-
- module SimR = {
-  proc f( pin: pin_t (*public inputs*)
-        , sin sin': sin_t (*secret inputs*): out_t = {
-    var r;
-    r <@ XtrR.f(pin, sin');
-    r <@ XtrI.f(pin, sin);
-    return r;
-  }
- }.
-
- The leakage-freeness property thus becomes:
-
- f_CT:
-  equiv [ XtrR.f ~ SimR.f
-        : ={pin, sin, XtrR.leakages} 
-          ==> ={res, XtrR.leakages}.
-
-*)
-
-module SimR = {
- proc randombytes_256(a a' (* ?secret? *): W8.t Array256.t): W8.t Array256.t = {
+module JI = {
+ proc main(pin : W64.t Array32.t, sin: unit) : W64.t Array32.t = {
   var r;
-  r <@  W64_SchnorrExtract_ct.Syscall.randombytes_256(a');
-  r <@  W64_SchnorrExtract.Syscall.randombytes_256(a);
-  return r;
- }
- proc bn_subc( a a' (*secret *): W64.t Array32.t
-             , b b' (*secret *): W64.t Array32.t) = {
-   var r;
-   r <@ XtrR.bn_subc(a', b');
-   r <@ XtrI.bn_subc(a, b);
-   return r;
- }
- proc bn_rsample(byte_z (*public *): W64.t Array32.t) = {
-   var r;
-   r <@ XtrR.bn_rsample(byte_z);
-   r <@ XtrI.bn_rsample(byte_z);
-   return r;
+  r <@ XtrI.bn_rsample(pin);
+  return r.`2;
  }
 }.
 
-require import DList.
-lemma randombytes_256_CT:
- equiv [ W64_SchnorrExtract_ct.Syscall.randombytes_256
-         ~ SimR.randombytes_256
-       : ={a, glob XtrR}
-         ==> ={res, glob XtrR}
-       ].
-proof.
-(* this is currently provable, but not sure if it should be assumed
- as an ASSUMPTION (should system-calls leak?) *)
-proc; inline*; simplify.
-wp; rnd; auto => />.
-apply dmap_ll.
-apply dmap_ll.
-apply dlist_ll.
-by apply W8.dword_ll.
-qed.
+lemma stateless_JI &m x: (glob JI){m} = x
+by done.
 
-(** The Jasmin's standard "constant-time" property
- establishes the independence of leakage wrt to the
- secret inputs \footnote{actually, the name was
- coined when the Jasmin language had no support for
- non-deterministic constructs -- we keep it for
- convenience.}.
-
- f_ct:
-  equiv [ XtrR.f ~ XtrR.f
-        : ={pin, XtrR.leakages} ==> ={XtrR.leakages} ]
-
- where [pin] are the public inputs of [f].
-
- Clearly, this property is a simple consequence of
- the [f_CT] property stated above. However, to some
- extent, the other direction is more insteresting, as
- the [f_ct] property is typically established fully
- automatically (resorting to the [sim] tactic). Hence,
- we observe that, in order to establish the [f_CT]
- property from the [f_ct] property, we are left with
- a slightly simpler version of [f_CT] that resembles
- a kind of Self-Composition:
-
- module SelfCompR = {
-  proc f( pin: pin_t (*public inputs*)
-        , sin: sin_t (*secret inputs*): out_t = {
-    var r;
-    r <@ XtrR.f(pin, sin);
-    r <@ XtrI.f(pin, sin);
-    return r;
-  }
- }.
-
- f_SC:
-  equiv [ XtrR.f ~ SelfCompR.f
-        : ={pin, sin, XtrR.leakages} 
-          ==> ={res, XtrR.leakages}.
-
- Intuively, [f_SC] does not bother in calling the
- "simulator" with dummy secret inputs. 
-*)
-
-module SelfCompR = {
- proc randombytes_256(a: W8.t Array256.t): W8.t Array256.t = {
+module JR = {
+ proc main(pin : W64.t Array32.t, sin: unit) : W64.t Array32.t = {
   var r;
-  r <@  W64_SchnorrExtract_ct.Syscall.randombytes_256(a);
-  r <@  W64_SchnorrExtract.Syscall.randombytes_256(a);
-  return r;
+  r <@ XtrR.bn_rsample(pin);
+  return r.`2;
  }
- proc bn_subc( a b: W64.t Array32.t) = {
-   var r;
-   r <@ XtrR.bn_subc(a, b);
-   r <@ XtrI.bn_subc(a, b);
-   return r;
- }
- proc bn_rsample(byte_z: W64.t Array32.t) = {
-   var r;
-   r <@ XtrR.bn_rsample(byte_z);
-   r <@ XtrI.bn_rsample(byte_z);
-   return r;
+ proc mainG(pin : W64.t Array32.t, sin: unit) : W64.t Array32.t * leakages_t = {
+  var r;
+  r <@ XtrR.bn_rsample(pin);
+  return (r.`2, XtrR.leakages);
  }
 }.
 
-(* we illustrate the previously mentioned observations
-  by instantiating them in with the [bn_subc] function. *)
-lemma bn_subc_ct_from_CT:
- equiv [ XtrR.bn_subc ~ SimR.bn_subc
-       : ={a, b, XtrR.leakages} ==> ={res, XtrR.leakages} ] =>
- equiv [ XtrR.bn_subc ~ XtrR.bn_subc
-       : ={XtrR.leakages} ==> ={XtrR.leakages} ].
+lemma proj_JR_JI:
+ equiv [ JR.main ~ JI.main
+       : ={pin, sin} ==> ={res} ].
 proof.
-move=> H_CT.
-proc*.
-transitivity{1} { r <@ SimR.bn_subc(a,a,b,b); }
- ( ={a, b, XtrR.leakages} ==> ={r,XtrR.leakages} )
- ( ={XtrR.leakages} ==> ={XtrR.leakages} ) => //.
-  move => /> &1 &2.
-  exists XtrR.leakages{2} a{1} b{1} => />.
- by call H_CT.
-inline SimR.bn_subc.
-wp; call{1} (: true ==> true).
- (* XtrI_bn_subc_ll *)
- proc; wp; while (0 < i <= 32) (32-i).
-  by move=> z; auto => /> * /#.
- by auto => /> * /#.
-by inline*; sim.
+proc; inline XtrR.bn_rsample XtrI.bn_rsample; simplify.
+sim.
+admit (* This should not occur! it appears that these extractions are not in sync... *).
 qed.
 
-lemma bn_subc_CT_from_ct_and_SC:
- equiv [ XtrR.bn_subc ~ XtrR.bn_subc
-       : ={XtrR.leakages} ==> ={XtrR.leakages} ] =>
- equiv [ XtrR.bn_subc ~ SelfCompR.bn_subc
-       : ={a, b, XtrR.leakages} ==> ={res, XtrR.leakages} ] =>
- equiv [ XtrR.bn_subc ~ SimR.bn_subc
-       : ={a, b, XtrR.leakages} ==> ={res, XtrR.leakages} ].
+lemma globJR:
+ equiv [ JR.main ~ JR.mainG
+       : ={pin,sin,glob JR}
+         ==> ={glob JR} /\ res{2} = (res{1},glob JR){2} ].
 proof.
-move=> H_ct H_SC.
-transitivity SelfCompR.bn_subc
- ( ={a, b, XtrR.leakages} ==> ={res, XtrR.leakages} )
- ( ={a, b, XtrR.leakages} ==> ={res, XtrR.leakages} ) => //.
- move => /> &1 &2 -> ->.
- by exists XtrR.leakages{2} (a{2},b{2}); auto.
-proc; simplify.
-call (: true); first by sim.
-by call H_ct; auto.
+proc*; inline JR.main JR.mainG.
+wp; call (: ={arg,glob JR} ==> ={res,glob JR}) => //.
+ by proc; sim.
+by auto.
 qed.
 
-
-(* in the case of [bn_rsample], this degenerate in
- trivial observations, as there are no secret
- inputs (just shown in one direction).                 *)
-lemma bn_rsample_CT_from_ct_and_SC:
- equiv [ XtrR.bn_rsample ~ XtrR.bn_rsample
-       : ={byte_z, XtrR.leakages} ==> ={XtrR.leakages} ] =>
- equiv [ XtrR.bn_rsample ~ SelfCompR.bn_rsample
-       : ={byte_z, XtrR.leakages} ==> ={res, XtrR.leakages} ] =>
- equiv [ XtrR.bn_rsample ~ SimR.bn_rsample
-       : ={byte_z, XtrR.leakages} ==> ={res, XtrR.leakages} ].
+lemma prMuE P pin sin &m:
+ Pr[ JR.main(pin,sin) @ &m : P (res,glob JR)]
+ = RealSeries.sum (fun (x:_*_) => Pr [JR.main(pin,sin) @ &m : P (res,glob JR) /\ res=x.`1 /\ (glob JR)=x.`2]).
 proof.
-move=> H_ct H_SC.
-transitivity SelfCompR.bn_rsample
- ( ={byte_z, XtrR.leakages} ==> ={res, XtrR.leakages} )
- ( ={byte_z, XtrR.leakages} ==> ={res, XtrR.leakages} ) => //.
- by move => /> &2; exists XtrR.leakages{2} arg{2}; auto.
+have ->: Pr[JR.main(pin, sin) @ &m : P (res,glob JR)]
+  = Pr[JR.mainG(pin, sin) @ &m : P res].
+ byequiv => //.
+ by conseq globJR => /> // /#.
+rewrite Pr [muE].
+apply RealSeries.eq_sum; move => [r l].
+rewrite eq_sym.
+by byequiv globJR => /> /#.
+qed.
+
+(* to prove CT on Bn_rsample, one could rely on...
+ (the interesting part is the proof of CC)        *)
+print Bn_rsample_CT.pinll_ct_CC_CT.
+
+end Bn_rsample.
+
+
+theory Bn_subc.
+
+clone import CT_Meta as Bn_subc_CT
+ with type pin_t <- unit,
+      type sin_t <- (W64.t Array32.t * W64.t Array32.t),
+      type out_t <- bool * W64.t Array32.t.
+
+module JI = {
+ proc main(pin : unit, sin: W64.t Array32.t * W64.t Array32.t) : bool * W64.t Array32.t = {
+  var r;
+  r <@ XtrI.bn_subc(sin.`1, sin.`2);
+  return r;
+ }
+}.
+
+lemma stateless_JI &m x: (glob JI){m} = x
+by done.
+
+module JR = {
+ proc main(pin : unit, sin: W64.t Array32.t * W64.t Array32.t) : bool * W64.t Array32.t = {
+  var r;
+  r <@ XtrR.bn_subc(sin.`1, sin.`2);
+  return r;
+ }
+ proc mainG(pin : unit, sin: W64.t Array32.t * W64.t Array32.t) : (bool * W64.t Array32.t) * leakages_t = {
+  var r;
+  r <@ XtrR.bn_subc(sin.`1, sin.`2);
+  return (r,XtrR.leakages);
+ }
+}.
+
+lemma proj_JR_JI:
+ equiv [ JR.main ~ JI.main
+       : ={pin, sin} ==> ={res} ].
+proof.
+proc; inline XtrR.bn_subc XtrI.bn_subc; simplify.
 by sim.
 qed.
 
-
-
-(** The case of deterministic functionalities.
-    ==========================================
-
- When [XtrI.f] is deterministic, the property of
- leakage-freeness ([f_CT] presented above) follows
- from the much simpler property [f_ct], that is,
- [f_SC] is a consequence of determinism of [f].
-
- Again, we illustrate the constructions and results
- with [bn_subc] function.                              *)
-
-(* a (trivial to prove) meta-property of the
- extraction mechanism                            *)
-lemma bn_subc_Iproj:
- equiv [ XtrI.bn_subc
-         ~ XtrR.bn_subc
-       : ={a,b} ==> ={res} ].
-proof. by proc; sim. qed.
-
-(* this is the (standard) constant-time characterisation *)
-lemma bn_subc_ct : 
- equiv [ XtrR.bn_subc
-         ~ XtrR.bn_subc
-       : ={XtrR.leakages} ==> ={XtrR.leakages} ].
-proof. by proc; sim. qed.
-
-(* determinism of a jasmin program *)
-lemma bn_subc_det:
- exists (f: W64.t Array32.t *  W64.t Array32.t ->  bool * W64.t Array32.t),
- forall _a _b,
- phoare [ XtrI.bn_subc
-        : a=_a /\ b=_b ==> res = f (_a, _b) ] = 1%r.
+lemma globJR:
+ equiv [ JR.main ~ JR.mainG
+       : ={pin,sin,glob JR}
+         ==> ={glob JR} /\ res{2} = (res{1},glob JR){2} ].
 proof.
-(* this follows from correctness of [bn_subc] *)
-admitted.
-
-(* some consequences of determinism (obs: probably,
- some of them are redundant -- just added when their
- need was felt...)                                 *)
-
-lemma bn_subc_det_ph:
- forall (f: W64.t Array32.t * W64.t Array32.t ->  bool * W64.t Array32.t),
- (forall _a _b,
-  phoare [ XtrI.bn_subc
-        : a=_a /\ b=_b ==> res = f (_a, _b) ] = 1%r)
- =>
- forall _a _b,
- phoare [ XtrR.bn_subc
-        : a=_a /\ b=_b ==> res = f (_a, _b) ] = 1%r.
-proof.
-move=> fsubc Hdet _a _b.
-bypr => &m [-> ->].
-have <-: Pr[XtrI.bn_subc(_a, _b) @ &m : res = fsubc (_a, _b)] 
-         = Pr[XtrR.bn_subc(_a, _b) @ &m : res = fsubc (_a, _b)].
- by byequiv bn_subc_Iproj.
-byphoare (: a=_a /\ b=_b ==> _) => //.
-by apply (Hdet _a _b).
+proc*; inline JR.main JR.mainG.
+wp; call (: ={arg,glob JR} ==> ={res,glob JR}) => //.
+ by proc; sim.
+by auto.
 qed.
 
-lemma bn_subc_det_h:
- forall (f: W64.t Array32.t * W64.t Array32.t ->  bool * W64.t Array32.t),
- (forall _a _b,
-  phoare [ XtrI.bn_subc
-         : a=_a /\ b=_b ==> res = f (_a, _b) ] = 1%r)
- => 
- forall _a _b,
- hoare [ XtrR.bn_subc: a=_a /\ b=_b ==> res = f (_a, _b) ].
+lemma prMuE P pin sin &m:
+ Pr[ JR.main(pin,sin) @ &m : P (res,glob JR)]
+ = RealSeries.sum (fun (x:_*_) => Pr [JR.main(pin,sin) @ &m : P (res,glob JR) /\ res=x.`1 /\ (glob JR)=x.`2]).
 proof.
-move=> fsubc Hfsubc _a _b.
-bypr => &m [-> ->].
-rewrite Pr [mu_not].
-have ->: Pr[XtrR.bn_subc(_a, _b) @ &m : true] = 1%r.
- (* bn_subc_ll *)
- byphoare (: true ==> true) => //=.
- proc; wp; while (0 < i <= 32) (32-i).
-  by move=> z; auto => /> * /#.
- by auto => /> * /#.
-have ->: Pr[XtrR.bn_subc(_a, _b) @ &m : res = fsubc (_a, _b)] = 1%r.
- by byphoare (bn_subc_det_ph fsubc Hfsubc _a _b).
-done.
+have ->: Pr[JR.main(pin, sin) @ &m : P (res,glob JR)]
+  = Pr[JR.mainG(pin, sin) @ &m : P res].
+ byequiv => //.
+ by conseq globJR => /> // /#.
+rewrite Pr [muE].
+apply RealSeries.eq_sum; move => [r l].
+rewrite eq_sym.
+by byequiv globJR => /> /#.
 qed.
 
-lemma bn_subc_det_pr:
- forall (f: W64.t Array32.t * W64.t Array32.t ->  bool * W64.t Array32.t),
- (forall _a _b,
-  phoare [ XtrI.bn_subc
-         : a=_a /\ b=_b ==> res = f (_a, _b) ] = 1%r)
- => 
- forall _a _b _l &m,
- Pr[ XtrR.bn_subc(_a,_b) @ &m: res = f (_a, _b) /\ XtrR.leakages = _l]
- = Pr[ XtrR.bn_subc(_a,_b) @ &m: XtrR.leakages = _l].
-proof.
-move=> fsubc Hfsubc _a _b _l &m.
-rewrite eq_sym Pr [mu_split (res = fsubc (_a, _b))] andbC; ring.
-byphoare (: a=_a /\ b=_b ==> _) => //.
-hoare.
-by conseq (bn_subc_det_h fsubc Hfsubc _a _b) => /> *.
-qed.
+(* to prove CT on Bn_subc, one could rely on...   *)
+print Bn_subc_CT.ct_det_CT.
 
-lemma bn_subc_det_eq:
- forall (f: W64.t Array32.t * W64.t Array32.t ->  bool * W64.t Array32.t),
- (forall _a _b,
-  phoare [ XtrI.bn_subc
-        : a=_a /\ b=_b ==> res = f (_a, _b) ] = 1%r)
- =>
- forall _a _b,
- equiv [ XtrR.bn_subc ~ XtrR.bn_subc
-       : a{2}=_a /\ b{2}=_b /\ ={a,b,XtrR.leakages} ==> ={res, XtrR.leakages} /\ res{2} = f (_a, _b)  ].
-proof.
-move=> fsubc Hfsubc _a _b.
-conseq (: ={XtrR.leakages} ==> ={XtrR.leakages}) (: a=_a /\ b=_b ==> res = fsubc (_a, _b)) (: a=_a /\ b=_b ==> res = fsubc (_a, _b)) => //.
-  by apply (bn_subc_det_h fsubc Hfsubc _a _b).
- by apply (bn_subc_det_h fsubc Hfsubc _a _b).
-by apply bn_subc_ct.
-qed.
+end Bn_subc.
 
-(** We can now state self-composition property [bn_subc_SC]
- as a consequence of [bn_subc_det], from which the
- [bn_subc_CT] property is derived.                       *)
-lemma bn_subc_SC:
- equiv [ XtrR.bn_subc
-         ~ SelfCompR.bn_subc
-       : ={a, b, glob XtrR}
-         ==> ={res, glob XtrR}
-       ].
-proof.
-proc*; simplify; inline SelfCompR.bn_subc.
-have [fsubc Hfsubc] := bn_subc_det.
-wp; ecall{2} (Hfsubc a0{2} b0{2}).
-exlim a{2}, b{2} => _a _b.
-have HH:= bn_subc_det_eq fsubc _ _a _b.
- by apply Hfsubc.
-by call HH; auto => /> &2.
-qed.
+theory TestComp.
 
-lemma bn_subc_CT:
- equiv [ XtrR.bn_subc
-         ~ SimR.bn_subc
-       : ={a, b, glob XtrR}
-         ==> ={res, glob XtrR}
-       ].
-proof.
-apply bn_subc_CT_from_ct_and_SC.
- by apply bn_subc_ct.
-by apply bn_subc_SC.
-qed.
-
-(* REMARK: we one finds that going through the [f_SC]
- property is an unnecessary detour, we can go directly
- from [f_ct] and [f_det] into [f_CT]...           *)
-lemma bn_subc_det_eq':
- forall (f: W64.t Array32.t * W64.t Array32.t ->  bool * W64.t Array32.t),
- (forall _a _b,
-  phoare [ XtrI.bn_subc
-        : a=_a /\ b=_b ==> res = f (_a, _b) ] = 1%r)
- =>
- forall _a _a' _b _b',
- equiv [ XtrR.bn_subc ~ XtrR.bn_subc
-       : a{1}=_a /\ a{2}=_a' /\ b{1}=_b /\ b{2}=_b' /\ ={XtrR.leakages} ==> ={XtrR.leakages} /\ res{1} = f (_a, _b) /\ res{2} = f (_a', _b') ].
-proof.
-move=> fsubc Hfsubc _a _a' _b _b'.
-conseq (: ={XtrR.leakages} ==> ={XtrR.leakages}) (: a=_a /\ b=_b ==> res = fsubc (_a, _b)) (: a=_a' /\ b=_b' ==> res = fsubc (_a', _b')) => //.
-  by apply (bn_subc_det_h fsubc Hfsubc _a _b).
- by apply (bn_subc_det_h fsubc Hfsubc _a' _b').
-by apply bn_subc_ct.
-qed.
-
-lemma bn_subc_CT':
- equiv [ XtrR.bn_subc
-         ~ SimR.bn_subc
-       : ={a, b, glob XtrR}
-         ==> ={res, glob XtrR}
-       ].
-proof.
-proc*; simplify; inline SimR.bn_subc.
-have [fsubc Hfsubc] := bn_subc_det.
-wp; ecall{2} (Hfsubc a0{2} b0{2}).
-exlim a{2}, a'{2}, b{2}, b'{2} => _a _a' _b _b'.
-have HH:= bn_subc_det_eq' fsubc _ _a _a' _b _b'.
- by apply Hfsubc.
-by call HH; auto => /> &2.
-qed.
+clone import CT_Comp as TestComp_CT
+ with type pin1_t <- W64.t Array32.t,
+      type pin2_t <- unit,
+      type sin1_t <- unit,
+      type sin2_t <- W64.t Array32.t,
+      type out1_t <- W64.t Array32.t,
+      type out2_t <- bool * W64.t Array32.t.
 
 
-(*
-
-  Now, we want to move towards the proof of the
- leakage-freeness property of [bn_rsample]. Following
- the previous discussion, we build on the [bn_rsample_ct]
- property which is trivial to prove.                     *)
-
-lemma bn_rsample_ct:
- equiv [ XtrR.bn_rsample
-         ~ XtrR.bn_rsample
-       : ={byte_z, XtrR.leakages} ==> ={XtrR.leakages}
-       ].
-proof. by proc; sim. qed.
-
-lemma bn_rsample_CT_from_SC:
- equiv [ XtrR.bn_rsample
-         ~ SelfCompR.bn_rsample
-       : ={byte_z, XtrR.leakages}
-         ==> ={res, XtrR.leakages} ] =>
- equiv [ XtrR.bn_rsample
-         ~ SimR.bn_rsample
-       : ={byte_z, XtrR.leakages}
-         ==> ={res, XtrR.leakages}
-       ].
-proof.
-apply bn_rsample_CT_from_ct_and_SC.
-by apply bn_rsample_ct.
-qed.
-
-(*
-
- In order to prove [bn_rsample_SC], we need to decouple
- the computation of results from the generation of the
- leakage. To do so, we start by spliting a sample
- from [0..R-1] through the probability of a given event.
- Specifically, we shall transform the rejection loop
- as follows:
-
-  ...
-  x <$ dR;	  (* [0..R-1] *) 
-  b <- pred_ev x; (* acceptance criteria *)
-  while (!b) {
-    ...
-    x <$ dR; 
-    b <- pred_ev x;
-  }
-  return x;
-
-  into:
-
-  ...
-  b <$ dbiased (mu dR pred_ev);
-  x <$ if b then dcond dR pred_ev
-            else dcond dR (predC pred_ev);
-  while (!b) {
-    ...
-    b <$ dbiased (mu dR pred_ev);
-    x <$ if b then dcond dR pred_ev
-              else dcond dR (predC pred_ev);
-  }
-
-
-  REMARK: notice that the above discussion critically
-  depends on the determinism of [bn_subc] (as [pred_ev]
-  is actually its functional description). In fact,
-  in order to apply this transformation, one should
-  previously rely on [bn_subc_CT] in order to recast
-  the (leaky) evaluation of [bn_subc] into a pure
-  function.
-*)
-
-require import DBool DProd.
-import Biased.
-
-abstract theory SampleEventSwap.
-
-type in_t.
-type out_t.
-
-module SampleEvent = {
- proc sample(i: in_t, d: in_t -> out_t distr, P: out_t -> bool): out_t * bool = {
-  var b, x;
-  x <$ d i;
-  b <- P x;
-  return (x, b);
- }
- proc sampleEv(i: in_t, d: in_t -> out_t distr, P: out_t -> bool): out_t * bool = {
-  var b, x;
-  b <$ dbiased (mu (d i) P);
-  x <$ if b then dcond (d i) P else dcond (d i) (predC P);
-  return (x, b);
- }
+module J2R = {
+ proc f1 = Bn_rsample.JR.main
+ proc f2 = Bn_subc.JR.main
 }.
 
-
-clone DLetSampling as LS with
- type t <- bool,
- type u <- out_t.
-
-equiv sample_sampleEv:
- SampleEvent.sample ~ SampleEvent.sampleEv:
- ={i, d, P} /\ is_lossless (d i){2} 
- ==> ={res}.
+lemma compCT:
+ equiv[ F.RSim(FComp(Bn_rsample.JI,Bn_subc.JI),
+               FComp(Bn_rsample.JR,Bn_subc.JR)).main 
+      ~ F.SimR(FComp(Bn_rsample.JI,Bn_subc.JI),
+               FComp(Bn_rsample.JR,Bn_subc.JR)).main
+      : ={pin,sin, glob Bn_rsample.JR, glob Bn_subc.JR}
+        ==> ={res, glob Bn_rsample.JR, glob Bn_subc.JR} ].
 proof.
-proc; simplify; wp.
-case: ((mu (d i) P){2}=0%r).
- seq 0 1: (#pre /\ !b{2}).
-  rnd{2}; auto => /> &m Hll Hb; split; first by apply dbiased_ll.
-  by move=> _ b; rewrite Hb dbiased0 supp_dunit.
- rnd; auto => /> &m Hll Hb0 Hb; split.
-  move=> xR; rewrite dcond_supp; move=> [Hx1 Hx2].
-  by rewrite dcond1E Hx2 /= mu_not Hll Hb0 /=.
- move => H xL Hx; split.
-  by rewrite dcond_supp Hx /predC /=; apply (eq0_mu (d{m} i{m})).
- by rewrite dcond_supp Hx /predC /= /#.
-case: ((mu (d i) P){2}=1%r).
- seq 0 1: (#pre /\ b{2}).
-  rnd{2}; auto => /> &m Hll _ Hb; split; first by apply dbiased_ll.
-  by move=> _ b; rewrite Hb dbiased1 supp_dunit.
- rnd; auto => /> &m Hll _ Hb1 Hb; split.
-  move=> xR; rewrite dcond_supp; move=> [Hx1 Hx2].
-  by rewrite dcond1E Hx2 Hb1.
- move => _ xL Hx; split.
-  rewrite dcond_supp Hx /=; apply (mu_in_weight _ (d{m} i{m})) => //.
-  by rewrite Hb1 Hll.
- by rewrite dcond_supp Hx /#.
-transitivity{1} { x <@ LS.SampleDLet.sample(dbiased (mu (d i) P), fun b=> if b then dcond (d i) P else dcond (d i) (predC P)); }
- (={i,d,P} /\ is_lossless (d i){2} /\ 0%r < (mu (d i) P){2} < 1%r
-  ==> ={x,i,d,P} /\ is_lossless (d i){2} /\ 0%r < (mu (d i) P){2} < 1%r)
- (={i,d,P} /\ is_lossless (d i){2} /\ 0%r < (mu (d i) P){2} < 1%r ==> ={x} /\ P{1} x{1}=b{2}) => //.
-  by move=> /> &m Hll Hbias1 Hbias2; exists P{m} d{m} i{m}; smt(mu_bounded).
- inline*; auto => /> &m Hll Hbias1 Hbias2; split.
-  move=> xR.
-  by rewrite -marginal_sampling_pred //.
- move => H xL HxL.
- rewrite supp_dlet.
- case: (P{m} xL) => bL.
-  exists true => /=.
-  rewrite supp_dbiased 1:/#.
-  by rewrite dcond_supp.
- exists false => /=.
- rewrite supp_dbiased 1:/#.
- by rewrite dcond_supp.
-transitivity{1} { x <@ LS.SampleDep.sample(dbiased (mu (d i) P), fun b=> if b then dcond (d i) P else dcond (d i) (predC P)); }
- (={i,d,P} /\ 0%r < (mu (d i) P){2} < 1%r ==> ={x,i,d,P} /\ 0%r < (mu (d i) P){2} < 1%r)
- (={i,d,P} /\ 0%r < (mu (d i) P){2} < 1%r ==> ={x} /\ P{1} x{1}=b{2}) => //.
-  by move=> /> &m Hll Hbias1 Hbias2; exists P{m} d{m} i{m}; auto.
- by symmetry; call LS.SampleDepDLet => //=.
-inline*; auto => /> &m Hbias1 Hbias2 b Hb xL.
-by case: (b) => Cb; rewrite dcond_supp /#.
+transitivity F.RSim(FComp(Bn_rsample.JI, Bn_subc.JI), FComp(Proc1(J2R), Proc2(J2R))).main
+ ( ={pin, sin, glob J2R} ==> ={res, glob J2R} )
+ ( ={pin, sin, glob J2R} ==> ={res, glob J2R} ) => //.
++ move => /> &1 &2 *.
+  by exists W64_SchnorrExtract_ct.M.leakages{2} (pin{1},sin{1}) => //.
++ proc.
+  inline FComp(Bn_rsample.JR, Bn_subc.JR).main.
+  inline FComp(Proc1(J2R), Proc2(J2R)).main.
+  by sim.
+transitivity F.SimR(FComp(Bn_rsample.JI, Bn_subc.JI), FComp(Proc1(J2R), Proc2(J2R))).main
+ ( ={pin, sin, glob J2R} ==> ={res, glob J2R} )
+ ( ={pin, sin, sin', glob J2R} ==> ={res, glob J2R} ) => //.
++ move => /> &1 &2 *.
+  by exists W64_SchnorrExtract_ct.M.leakages{2} (pin{1},sin{1},sin'{2}) => /> //.
++ apply (Compositionality J2R Bn_rsample.JI Bn_subc.JI _ _ _ _ _ _).
+  (* AXIOMS *)
+  - exact Bn_rsample.stateless_JI.
+  - exact Bn_subc.stateless_JI.
+  - exact Bn_rsample.proj_JR_JI.
+  - exact Bn_subc.proj_JR_JI.
+  - exact Bn_rsample.prMuE.
+  - exact Bn_subc.prMuE.
+  (* PREMISES *)
+  - admit (* CT-1 *). 
+  - admit (* CT-2 *).
++ proc.
+  inline FComp(Bn_rsample.JR, Bn_subc.JR).main.
+  inline FComp(Proc1(J2R), Proc2(J2R)).main.
+  inline Proc1(J2R).main Proc2(J2R).main.
+  by sim.
 qed.
 
-end SampleEventSwap.
-
-(*
-  Then, we need to reshape the samplings in the
-  RejectionLoop. Specifically, we transform:
-
-  ...
-  b <$ dbiased (mu dR pred_ev);
-  x <$ if b then dcond dR pred_ev
-            else dcond dR (predC pred_ev);
-  while (!b) {
-    ...
-    b <$ dbiased (mu dR pred_ev);
-    x <$ if b then dcond dR pred_ev
-              else dcond dR (predC pred_ev);
-  }
-
-  into:
-
-  ...
-  b <$ dbiased (mu dR pred_ev);
-            else dcond dR (predC pred_ev);
-  while (!b) {
-    x <$ dcond dR (predC pred_ev);
-    ...
-    b <$ dbiased (mu dR pred_ev);
-  }
-  x <$ dcond dR pred_ev;
-  return x;
-
-  We resort to EC's PROM library for this eager/lazy
-  sampling rasoning.
+end TestComp.
 *)
-
-
-abstract theory RejectionLoop.
-
-type t.
-type in_t.
-
-op dt: in_t -> t distr.
-op p : t -> bool.
-
-
-module type AdvLoop = {
-  proc init(xin: in_t): unit
-  proc body(x: t): unit
-}.
-
-module RejLoop(L:AdvLoop) = {
-  proc loop1 (xin: in_t) = {
-    var x, b;
-    L.init(xin);
-    x <$ dt xin;
-    b <- p x;
-    while (! b) {
-      L.body(x);
-      x <$ dt xin;
-    }
-    return x;
-  }
-  proc loop2 (xin: in_t) = {
-    var x, b;
-    L.init(xin);
-    b <$ dbiased (mu (dt xin) p);
-    while (!b) {
-      x <$ dcond (dt xin) (predC p);
-      L.body(x);
-      b <$ dbiased (mu (dt xin) p);
-    }
-    x <$ dcond (dt xin) p;
-    return x;
-  }
-}.
-
-
-
-require import PROM SmtMap.
-
-clone import PROM.FullRO as ROx with
-    type in_t    <- in_t*bool,
-    type out_t   <- t, 
-    type d_in_t  <- in_t,
-    type d_out_t <- t,
-    op   dout    <- fun (y:_*_) => if y.`2
-                                   then dcond (dt y.`1) p
-                                   else dcond (dt y.`1) (predC p)
-  proof *.
-
-module RejLoop_D (L:AdvLoop) (O: RO) = {
- proc distinguish(xin: in_t): t = {
-  var b, x;
-  L.init(xin);
-  b <$ dbiased (mu (dt xin) p);
-  O.sample(xin,b);
-  while (!b) {
-    x <@ O.get(xin,b);
-    O.rem(xin,b);
-    L.body(x);
-    b <$ dbiased (mu (dt xin) p);
-    O.sample(xin,b);
-  }
-  x <@ O.get(xin,b);
-  (* O.rem(xin,b); *)
-  return x;
- }
-}.
-
-section.
-
-declare module L <: AdvLoop {-RO, -LRO}.
-
-module RejLoopD = RejLoop_D(L).
-
-
-equiv loop1_loop2:
- RejLoop(L).loop1 ~ RejLoop(L).loop2:
- ={xin, glob L}
- ==> ={res, glob L}.
-proof.
-proc*.
-transitivity{1}
- { RO.init();
-   r <@ RejLoopD(RO).distinguish(xin); }
- ( ={xin, glob L} ==> ={xin, r, glob L} )
- ( ={xin, glob L} ==> ={r, glob L} ) => //.
-+ by move=> /> &2; exists (glob L){2} xin{2} => />.
-+ inline RejLoop(L).loop1 RejLoopD(RO).distinguish.
-  inline RO.sample RO.get.
-  seq 2 3: (={xin, xin0, glob L}).
-   by call (: true); inline*; auto => />.
-  seq 2 5: (={xin, xin0, b, glob L} /\ (RO.m.[(xin0,b)]){2}=Some x{1}).
-   admit (*SampleEvSwap*).
-  seq 1 1: (={xin, xin0, b, glob L} /\ !b{2} /\ (RO.m.[(xin0,b)]){2}=Some x{1}).
-   admit (* loop *).
-  wp; rnd{2}; auto => /> &1 &2 Hb Hm; split.
-   admit (*ll*).
-  move=> _ ?? />.
-  have->/=: (xin0{2}, false) \in RO.m{2} by smt().
-  by rewrite Hm /=.
-transitivity{1}
- { LRO.init();
-   r <@ RejLoopD(LRO).distinguish(xin); }
- ( ={xin, glob L} ==> ={xin, r, glob L} )
- ( ={xin, glob L} ==> ={r, glob L} ) => //.
-+ by move=> /> &2; exists (glob L){2} xin{2} => />.
-+ admit (* need to sort out module restrictions...
-           (hopefully, without droping the RejLoop abstraction...)
-  call (FullEager.RO_LRO_D RejLoopD).
-  *).
-inline RejLoop(L).loop2 RejLoopD(LRO).distinguish.
-inline LRO.sample LRO.get.
-admit.
-qed.
-
-end section.
-
-print loop1_loop2.
-
-end RejectionLoop.
-
-
-(*
-  Finally, we observe that the result of [bn_rsample]
-  is now fully detached from the leakage generation,
-  allowing us to establish the SC property:
-
-  (* XtrR.bn_rsample *)
-  ...
-  b <$ dbiased (mu dR pred_ev);
-            else dcond dR (predC pred_ev);
-  while (!b) {
-    x <$ dcond dR (predC pred_ev);
-    ...
-    b <$ dbiased (mu dR pred_ev);
-  }
-  x <$ dcond dR pred_ev;
-
-  (* XtrI.bn_rsample *)
-  x <$ dcond dR pred_ev;
-
-  return x;
-*)
-
-(*...*)
-
-(* The code of XtrR.bn_rsample:
-
-  proc bn_rsample(byte_z : W64.t Array32.t) : int * W64.t Array32.t = {
-    var aux_5 : bool;
-    var aux_4 : bool;
-    var aux_3 : bool;
-    var aux_2 : bool;
-    var aux_1 : bool;
-    var aux : int;
-    var aux_6 : W64.t;
-    var aux_7 : W8.t Array256.t;
-    var aux_0 : W64.t Array32.t;
-    var i : int;
-    var byte_p : W64.t Array32.t;
-    var cf : bool;
-    var _byte_p : W64.t Array32.t;
-    var byte_q : W64.t Array32.t;
-    var _0 : bool;
-    var _1 : bool;
-    var _2 : bool;
-    var _3 : bool;
-    var _4 : W64.t;
-    
-    _byte_p <- witness;
-    byte_p <- witness;
-    byte_q <- witness;
-    M.leakages <- (LeakAddr [] :: M.leakages)%List;
-    aux <- 0;
-    i <- aux;
-    M.leakages <- (LeakAddr [] :: M.leakages)%List;
-    aux_0 <@ M(SC).bn_set0(byte_p);
-    byte_p <- aux_0;
-    M.leakages <- (LeakAddr [] :: M.leakages)%List;
-    (aux_5, aux_4, aux_3, aux_2, aux_1, aux_6) <- set0_64_;
-    _0 <- aux_5;
-    cf <- aux_4;
-    _1 <- aux_3;
-    _2 <- aux_2;
-    _3 <- aux_1;
-    _4 <- aux_6;
-    M.leakages <- (LeakCond (!cf) :: LeakAddr [] :: M.leakages)%List;
-    while (!cf){
-      M.leakages <- (LeakAddr [] :: M.leakages)%List;
-      aux_0 <- byte_p;
-      _byte_p <- aux_0;
-      M.leakages <- (LeakAddr [] :: M.leakages)%List;
-      aux_7 <@
-        SC.randombytes_256((init (fun (i_0 : int) => get8 (init64 (fun (i_0_0 : int) => _byte_p.[i_0_0])) i_0))%Array256);
-      byte_p <- (init (fun (i_0 : int) => get64 (init8 (fun (i_0_0 : int) => aux_7.[i_0_0])) i_0))%Array32;
-      M.leakages <- (LeakAddr [] :: M.leakages)%List;
-      aux_0 <@ M(SC).bn_copy(byte_p);
-      byte_q <- aux_0;
-      M.leakages <- (LeakAddr [] :: M.leakages)%List;
-      (aux_5, aux_0) <@ M(SC).bn_subc(byte_q, byte_z);
-      cf <- aux_5;
-      byte_q <- aux_0;
-      M.leakages <- (LeakAddr [] :: M.leakages)%List;
-      aux <- i + 1;
-      i <- aux;
-      M.leakages <- (LeakCond (!cf) :: LeakAddr [] :: M.leakages)%List;
-    }
-    
-    return (i, byte_p);
-  }
-*)
-
-
-abstract theory Bn_subc_det.
-
-op fsubc: W64.t Array32.t *  W64.t Array32.t ->  bool * W64.t Array32.t.
-
-axiom subc_det _a _b:
- phoare [ XtrI.bn_subc
-        : a=_a /\ b=_b ==> res = fsubc (_a, _b) ] = 1%r.
-
-
-(*...*)
-
-end Bn_subc_det.
-
-
-
-
-(* TODO: link with low-level Defs. *)
